

题目 1. For each of the following s_n , determine s_n and its ordinary generating function.

$$1. s_n := \sum_{k=0}^n k \binom{n}{k};$$

$$2. s_n := \sum_{k=0}^n \binom{m+k}{m};$$

$$3. s_n := \sum_{k=0}^n \binom{n-k}{k}.$$

解答. 1.

Notice that $k \binom{n}{k} = n \binom{n-1}{k-1}$. Hence $s_n = n \sum_{k=0}^{n-1} \binom{n-1}{k-1} = n 2^{n-1}$.

Let $F(x) := \sum_{n=0}^{\infty} s_n x^n = x \sum_{n=0}^{\infty} n (2x)^{n-1} = x D(\sum_{n=0}^{\infty} (2x)^n) = \frac{x}{(1-2x)^2}$.

2. Let $F_m(x) := \sum_{n=0}^{\infty} s_n x^n$. Then $F_m(x) = 1 + \sum_{n=1}^{\infty} \left(s_{n-1} + \binom{m+n}{m} \right) x^n = x F_m(x) + \sum_{n=0}^{\infty} \binom{m+n}{m} x^m$

Let $G_m(x) := \sum_{n=0}^{\infty} \binom{m+n}{n} x^n$.

Then $G_m(x) = \sum_{n=0}^{\infty} \binom{m+n}{n} x^n = 1 + \sum_{n=1}^{\infty} \binom{m+n-1}{n} x^n + \sum_{n=1}^{\infty} \binom{n+m-1}{n-1} x^n = x G_m(x) + \sum_{n=0}^{\infty} \binom{m-1+n}{n} x^n = x G_m(x) + G_{m-1}(x)$.

Since $G_0(x) = \frac{1}{1-x}$, $G_m(x) = \left(\frac{1}{1-x} \right)^{m+1}$. Hence $F_m(x) = \left(\frac{1}{1-x} \right)^{m+2}$.

When $n \geq 2$, $s_n = 1 + \binom{m+1}{1} + \binom{m+2}{2} + \dots + \binom{m+n}{n} = \binom{m+1}{0} + \binom{m+1}{1} + \binom{m+2}{2} + \dots + \binom{m+n}{n} = \binom{m+2}{1} + \binom{m+2}{2} + \dots + \binom{m+n}{n} = \binom{m+3}{2} + \binom{m+3}{3} + \dots + \binom{m+n}{n} = \binom{m+n+1}{n}$.

3. We use the trick of swapping the summation order.

Let $F(x) := \sum_{n=0}^{\infty} s_n x^n = \sum_{n=0}^{\infty} \sum_{k=0}^n \binom{n-k}{k} x^n = \sum_{k=0}^{\infty} \sum_{n \geq k} \binom{n-k}{k} x^n = \sum_{k=0}^{\infty} \frac{1}{k!} x^k \sum_{n \geq k} (n-k)(n-k-1) \dots (n-k-k+1) x^{n-k} = \sum_{k=0}^{\infty} x^{2k} D^k \left(\sum_{n \geq k} x^{n-k} \right) = \sum_{k=0}^{\infty} \frac{x^{2k}}{(1-x)^{k+1}} = \frac{1}{1-x} \frac{1}{1 - \frac{x^2}{1-x}} = \frac{1}{1-x-x^2}$.

so s_n = the Fibonacci numbers.

题目 2. Let S be a *colored set*, i.e., there exists a mapping $c: S \rightarrow C$, where the elements of C are called *colors*. A *rainbow subset* of a colored set is a subset in which every element has a distinct color.

Note that a rainbow subset does **not necessarily** contain all colors in C . Let S be a fixed colored set, where

$$C := [k] = \{1, 2, \dots, k\}.$$

Let $n_i := |c^{-1}(i)|$, i.e., the number of elements of color i . Define f_m to be the number of rainbow subsets of S of size m .

1. Find the generating function of f_m . (You do not need to express it in a closed simple form, but simplify as much as possible.)
2. Suppose $n_1 = n_2 = \dots = n_k = n$. Find f_m .
3. Suppose $n_1 = 1, n_2 = 2, \dots, n_k = k$. Find f_m .

解答. 1.

By the question, each color has n_i choices, hence the multiplication factor should be $(1 + n_i z_i)$. Hence the generating function should be $\prod_{i=1}^k (1 + n_i z_i)$. And We specilazation $z_i = z$. Hence the answer is $\prod_{i=1}^k (1 + n_i z)$.

2. Too silly. $\binom{m}{k} n^k$.

同一行第一类斯特林数的计算

类似第二类斯特林数，我们构造同行第一类斯特林数的生成函数，即

$$F_n(x) = \sum_{i=0}^n \begin{bmatrix} n \\ i \end{bmatrix} x^i$$

根据递推公式，不难写出

$$F_n(x) = (n-1)F_{n-1}(x) + xF_{n-1}(x)$$

于是

$$F_n(x) = \prod_{i=0}^{n-1} (x+i) = \frac{(x+n-1)!}{(x-1)!}$$

3.

[\(hlink|斯特林数 - OI Wiki|\)](#)

[\(hlink|https://oi-wiki.org/math/combinatorics/stirling/\)](https://oi-wiki.org/math/combinatorics/stirling/)

So the answer is the first stirling number.

题目 3. Let $R = \mathbb{C}[x]$, and $E = \text{End}_{\mathbb{C}}(R)$. Consider the following two elements in E :

$$z: p \mapsto xp, \quad D: p \mapsto \frac{d}{dx} p.$$

All the following equations are regarded as equalities in E .

1. Prove that $Dz^k - z^k D = k z^{k-1}$. Here k is a natural number.
2. Find $a_{n,k}$ such that

$$(zD)^n = \sum_{k=0}^n a_{n,k} z^k D^k.$$

3. Find $b_{n,k}$ such that

$$z^n D^n = \sum_{k=0}^n b_{n,k} (zD)^k.$$

4. Find $c_{n,i,j}$ such that

$$(z + D)^n = \sum_{i=0}^n \sum_{j=0}^n c_{n,i,j} z^i D^j.$$

解答. 1.

$\forall f \in \mathbb{C}[x]$, suppose $f = \sum_{n=0}^{\infty} a_n x^n$. $Dz^k(f) = \sum_{n=0}^{\infty} (n+k) a_n x^{n+k-1}$. $z^k D(f) = \sum_{n=0}^{\infty} n a_n x^{n+k-1}$.

2. $(zD)^{n+1} = zD(\sum_{k=0}^n a_{n,k} z^k D^k) = \sum_{k=0}^n a_{n,k} z(z^k D + k z^{k-1} D) D^k = \sum_{k=0}^n a_{n,k} z^{k+1} D^{k+1} + \sum_{k=0}^n a_{n,k} k z^k D^k$

Hence $a_{n+1} = a_{n,k-1} + k a_{n,k}$.

That is still the first stirling number.

3. By the notes (you can see it in the following) . $(-1)^{n-k} S(n, k)$.

题目 4. Let $f(n)$ be the number of partitions of n such that for every k , k occurs in the partition at most k times. Let $g(n)$ be the number of partitions of n such that no part has the form $k(k+1)$ (i.e. no parts equal $2, 6, 12, \dots$). Show that $f(n) = g(n)$.

解答. Just Let $F(x) := \sum_{n=0}^{\infty} f(n) x^n$ and $G(x) := \sum_{n=0}^{\infty} g(n) x^n$. By the question, $G(x) = \prod_{i \neq k(k+1), i \geq 1} \frac{1}{1-x^i}$.

$$F(x) = (1+x)(1+x^2+x^4)(1+x^3+x^6+x^9) \dots = \prod_{i=1}^{\infty} \frac{1-x^{i(i+1)}}{1-x^i}.$$

Problem 5

Let $f_k(m, n)$ denote the number of $m \times n$ $\{0, 1\}$ -matrices with exactly k ones such that **each row contains at least one 1**.

Let $g_k(m, n)$ denote the number of $m \times n$ $\{0, 1\}$ -matrices with exactly k ones such that **each row and each column contain at least one 1**.

(i) Find the generating function of $f_k(m, n)$ with respect to k , that is, find

$$\sum_{k \geq 0} f_k(m, n) z^k.$$

(ii) Find the generating function of $g_k(m, n)$ with respect to k , that is, find

$$\sum_{k \geq 0} g_k(m, n) z^k.$$

(iii) Prove that

$$\sum_{m, n, k \geq 0} g_k(m, n) z^k \frac{x^m}{m!} \frac{y^n}{n!} = e^{-x-y} \sum_{i, j \geq 0} (1+z)^i \frac{x^i}{i!} \frac{y^j}{j!}.$$

解答. (i)

By the question, the generating function should be written as $F_n = \prod_{i=1}^m \left(x + \binom{n}{2} x^2 + \binom{n}{3} x^3 + \dots + \binom{n}{n} x^n \right) = ((1+x)^n - 1)^m$.

(ii)

We use the PIE

$$\left| \bigcup_{i=1}^n A_i \right| = \sum_{\emptyset \neq J \subseteq \{1, \dots, n\}} (-1)^{|J|+1} \left| \bigcap_{j \in J} A_j \right|$$

$$\left| \bigcap_{i=1}^n \overline{A_i} \right| = |S| - \sum_{i=1}^n |A_i| + \sum_{1 \leq i < j \leq n} |A_i \cap A_j| - \dots + (-1)^n |A_1 \cap \dots \cap A_n|.$$

Set $S = \{m \times n \text{ matrices with at least one 1 in every row}\}$.

$E_i = \{E_i \in S : E_i \text{ has no 1 in the } i \text{ column}\}$.

Then we use the second formula.

So $\sum_{k \geq 0} g_k(m, n) z^k = F_n + \sum_{i=1}^n \binom{n}{i} (-1)^i F_{n-i}$.

注记 1. Three polynomial bases

- Ordinary powers: x^n .
- Falling factorials:

$$x^{\underline{n}} = x(x-1)\cdots(x-n+1), x^{\underline{0}} = 1.$$

- Rising factorials:

$$x^{\overline{n}} = x(x+1)\cdots(x+n-1), x^{\overline{0}} = 1,$$

with the basic relation $x^{\overline{n}} = (-1)^n (-x)^{\underline{n}}$.

1) Ordinary powers \leftrightarrow Falling factorials (Stirling numbers)

- Expand ordinary powers in the falling basis

$$x^n = \sum_{k=0}^n S(n, k) x^{\underline{k}}$$

where $S(n, k)$ are the **Stirling numbers of the second kind** (partitions of an n -set into k nonempty blocks).

- Expand falling factorials in ordinary powers

$$x^{\underline{n}} = \sum_{k=0}^n s(n, k) x^k$$

where $s(n, k)$ are the **(signed) Stirling numbers of the first kind**, and

$s(n, k) = (-1)^{n-k} \begin{bmatrix} n \\ k \end{bmatrix}$ with $\begin{bmatrix} n \\ k \end{bmatrix}$ the **unsigned** ones.

2) Ordinary powers \leftrightarrow Rising factorials

- Expand ordinary powers in the rising basis

$$x^n = \sum_{k=0}^n (-1)^{n-k} S(n, k) x^{\overline{k}}$$

(obtained from $x^{\overline{k}} = (-1)^k (-x)^{\underline{k}}$).

- Expand rising factorials in ordinary powers

$$x^{\overline{n}} = \sum_{k=0}^n \begin{bmatrix} n \\ k \end{bmatrix} x^k$$

where $\begin{bmatrix} n \\ k \end{bmatrix} = (-1)^{n-k} s(n, k)$ are the **unsigned Stirling numbers of the first kind**.

3) Falling factorials \leftrightarrow Rising factorials (Lah numbers)

The change of basis between the two factorial bases is governed by the **Lah numbers**

$$L(n, k) = \binom{n-1}{k-1} \frac{n!}{k!} (1 \leq k \leq n).$$

- **Rising in terms of falling**

$$x^{\bar{n}} = \sum_{k=1}^n L(n, k) x^{\underline{k}}$$

- **Falling in terms of rising**

$$x^{\underline{n}} = \sum_{k=1}^n (-1)^{n-k} L(n, k) x^{\bar{k}}$$

4) Quick table ($n \leq 4$)

- $x^{\underline{1}} = x, x^{\underline{2}} = x^2 - x, x^{\underline{3}} = x^3 - 3x^2 + 2x, x^{\underline{4}} = x^4 - 6x^3 + 11x^2 - 6x.$
- $x^{\bar{1}} = x, x^{\bar{2}} = x^2 + x, x^{\bar{3}} = x^3 + 3x^2 + 2x, x^{\bar{4}} = x^4 + 6x^3 + 11x^2 + 6x.$

These identities give a complete and practical conversion kit among the three bases.